some more work

src/AwsCryptographicMaterialProviders/Client.dfy
@@ -7,6 +7,8 @@ include "../Util/UTF8.dfy"
 include "../Crypto/AESEncryption.dfy"
 include "Keyrings/RawAESKeyring.dfy"
 include "CMMs/DefaultCMM.dfy"
+include "Materials.dfy"
+include "AlgorithmSuites.dfy"
 
 module
   {:extern "Dafny.Aws.Crypto.MaterialProviders.Client"}
@@ -20,18 +22,48 @@ module
   import AESEncryption
   import RawAESKeyring
   import DefaultCMM
+  import AlgorithmSuites
+  import Materials
+
+  // This file is the entry point for all Material Provider operations.
+  // There MUST NOT be any direct includes to any other files in this project.
+  // The `constructor` for this `Client` is how any default
+  // or unanticipated behavior change will be made.
+  // Further anyone implementing their own CMM or Keyring
+  // needs to use this `Client` to access the required functions
+  // to ensure correctness of their components.
+  // This means that anything needed for the `Keyring` or `CMM` traits.
 
   export
-    provides Crypto
-    provides AwsCryptographicMaterialProvidersClient.CreateRawAesKeyring
-    provides AwsCryptographicMaterialProvidersClient.CreateDefaultCryptographicMaterialsManager
+    // Modules
+    provides Crypto, AlgorithmSuites, Materials
+    // Class
     reveals AwsCryptographicMaterialProvidersClient
+    // Functions
+    reveals SpecificationClient, SpecificationClient.GetSuite
+    // Class Members
+    provides
+      AwsCryptographicMaterialProvidersClient.CreateRawAesKeyring,
+      AwsCryptographicMaterialProvidersClient.CreateDefaultCryptographicMaterialsManager
+
+  datatype SpecificationClient = SpecificationClient(
+    // Whatever top level closure is added to the constructor needs to be added here
+  )
+  {
+    function method GetSuite(
+      id: Crypto.AlgorithmSuiteId
+    ):
+      (res: AlgorithmSuites.AlgorithmSuite)
+      ensures res.id == id
+    {
+      AlgorithmSuites.GetSuite(id)
+    }
+  }
 
   class AwsCryptographicMaterialProvidersClient
     extends Crypto.IAwsCryptographicMaterialsProviderClient
   {
     constructor () {}
-
     method CreateRawAesKeyring(input: Crypto.CreateRawAesKeyringInput)
       returns (res: Crypto.IKeyring)
     {
@@ -77,6 +109,10 @@ module
     {
         return new DefaultCMM.DefaultCMM.OfKeyring(input.keyring);
     }
+// Materials.EncryptionMaterialsTransitionIsValid(
+// Materials.DecryptionMaterialsTransitionIsValid(
+// Materials.EncryptionMaterialsWithPlaintextDataKey(
+// Materials.DecryptionMaterialsWithPlaintextDataKey(
   }
 
 }
